fixed some type-checking issues
even after lots of fuel, fstar fails to recongnize delta equality of some type definitions, and produces strange errors.

examples/low-level/sieve.fst
@@ -1,11 +1,10 @@
 (*--build-config
     options:--admit_fsi Set;
     variables:LIB=../../lib;
-    other-files:$LIB/ext.fst $LIB/set.fsi $LIB/heap.fst $LIB/st.fst $LIB/array.fst $LIB/list.fst  stack.fst listset.fst st3.fst example1.fst  $LIB/seq.fsi $LIB/seq.fst
+    other-files:$LIB/ext.fst $LIB/set.fsi $LIB/heap.fst $LIB/st.fst $LIB/list.fst  stack.fst listset.fst st3.fst example1.fst
   --*)
 
 module ScopedWhile3
-open Seq
 open StructuredMem
 open Heap
 open Stack
@@ -13,7 +12,6 @@ open Set
 open Prims
 open List
 open ListSet
-open Array
 
 
 val divides : pos -> nat -> Tot bool
@@ -35,32 +33,51 @@ type isPrime n = forall (m:nat). ((2<m /\ m<n) ==> not (divides m n))
 (*Suppose we are at the m^th iteration in the outer loop*)
 
 (*in a simplified version both inner and outer guards are same; just different variables*)
-type guardLC (n:nat) (li : ref nat) (m:smem) =
-  (refExistsInMem li m) && (((loopkupRef li m) < n))
+type guardLC (n:nat) (li : ref nat) (lo : ref nat)
+(m:smem) =
+  (refExistsInMem li m) && (refExistsInMem lo m) && (((loopkupRef li m) * (loopkupRef lo m) < n))
 
-val guard :  n:nat -> li:(ref nat)  -> unit
-  -> whileGuard (fun m -> b2t (refExistsInMem li m))
-                (guardLC n li)
-let guard n li u = (memread li < n)
+val guard :  n:nat -> li:(ref nat) -> lo:(ref nat)  -> unit
+  -> whileGuard (fun m ->  (refExistsInMem li m) /\ (refExistsInMem lo m))
+                (guardLC n li lo)
+let guard n li lo u = (memread li * memread lo < n)
 (* the guard of a while loop is not supposed to change the memory*)
 
-type vector (a:Type) (n:nat) = ll:(seq a){length ll=n}
+type vector (a:Type) (n:nat) = (k:nat{k<n}) -> Tot a
 
-type refBitVector (n:nat) = ref (ll:seq bool{length ll=n})
+type refBitVector (n:nat) = ref (vector bool n)
 
-val marked : n:nat -> ll:seq bool{length ll=n} -> nat -> Tot bool
-let marked n ll m = (index ll m)
+(*cannot make n implcit, because the typechecker usually canNOT figure it out from f*)
+val marked : n:nat -> (vector bool n) -> m:nat{m<n} -> Tot bool
+let marked n f m = (f m)
 
 (*#set-options "--initial_fuel 100 --max_fuel 10000 --initial_ifuel 100 --max_ifuel 10000"*)
 (*delta-folding vector creates a wierd error; see below*)
 
+(*nmult, for times when the typechecker confuses nats and ints*)
+val nmult : nat -> nat -> Tot nat
+let nmult n m = n*m
+
+val bforall : (nat -> Tot bool) -> nat -> Tot bool
+let rec bforall f bound =
+match bound with
+| 0 -> true
+| _ -> (f bound) && (bforall f (bound -1))
+
 (*li is the counter for the inner loop; lo is for the outer one*)
 (*the inner loop invariant says that cells lo*0, lo*1, lo*2 ....lo*(li-1) (first li multiples of lo) are marked.*)
-type  innerLoopInv (n:nat) (lo: ref nat) (li : ref nat) (res :  ref (ll:seq bool{length ll=n})) (m:smem) =
-  (refExistsInMem res m)
-  /\ (refExistsInMem li m)
-  /\ (refExistsInMem lo m)
-  /\ (forall (k:nat). k<(loopkupRef li m)  ==> marked n (loopkupRef res m) ((loopkupRef lo m)*k))
+
+#set-options "--initial_fuel 100 --max_fuel 1000 --initial_ifuel 100 --max_ifuel 1000"
+
+type  innerLoopInv (n:nat) (lo: ref nat) (li : ref nat) (res:ref ((k:nat{k<n}) -> Tot bool)) (m:smem) =
+  (guardLC n li lo m)
+  /\ (refExistsInMem res m)
+  /\ (forall (k:nat).
+        (k < (loopkupRef li m)) ==> (marked n (loopkupRef res m) ((loopkupRef lo m)*k)))
+
+val mark : n:nat -> ((k:nat{k<n}) -> Tot bool) -> index:nat{index<n} -> Tot ((k:nat{k<n}) -> Tot bool)
+let mark n f index =
+  (fun indx -> if (indx= index) then true else f indx)
 
 (*we are inside a loop, so, we have a fresh stack at each iteration of the loop.
  we store li there. creating li is a part of the outer loop*)
@@ -68,10 +85,11 @@ type  innerLoopInv (n:nat) (lo: ref nat) (li : ref nat) (res :  ref (ll:seq bool
 val innerLoop : n:nat
   -> lo: ref nat
   -> li : ref nat
-  -> res : ref  (ll:seq bool{length ll=n})
-  -> SST unit (fun m -> refExistsInMem lo m /\ refExistsInMem res m /\ (mreads li 0 m))
-              (fun _ _ m1 -> refExistsInMem lo m1 /\ refExistsInMem res m1 /\  refExistsInMem lo m1
-                  /\ (forall (k:nat). k<n  ==> marked n (loopkupRef res m1) ((loopkupRef lo m1)*k)))
+  -> res : ref ((k:nat{k<n}) -> Tot bool)
+  -> SST unit (fun m -> refExistsInMem lo m /\ refExistsInMem res m /\ (mreads li 0 m) /\ ~(li=lo))
+              (fun _ _ m1 -> refExistsInMem lo m1 /\ refExistsInMem res m1 /\  refExistsInMem li m1
+                  /\ (forall (k:nat). (k * (loopkupRef lo m1) < n)  ==> marked n (loopkupRef res m1) ((loopkupRef lo m1)*k))
+                  )
 
 (*let innerLoop n lo li res =
   scopedWhile
@@ -83,7 +101,10 @@ val innerLoop : n:nat
       let lov = memread lo in
       let resv = memread res in
       memwrite li (liv+1);
-      memwrite res (Seq.upd resv lov*li))*)
+      memwrite res (mark n resv (lov * liv)))*)
+
+      (*let resv2=memread res in
+      assert (resv2==resv);*)
 
 (*val innerLoopBody :
   n:nat -> lo:(ref pos) -> li:(ref pos) -> res:(ref (ll:seq bool{length ll=n}))
